1. -2 + (-5)

= -2 + (-5)
= -2 - 5
= -7

2. 1 - (-3)

= 1 - (-3)
= 1 + 3
= 4

3. 8 - 17

= 8 - 17
= -9  

4. -4 - (-3)

= -4 - (-3)
= -4 + 3
= -1


5. 6(-8)

= 6(-8)
= 6 * -8
= -48


6. (-3)(6)

= (-3)(6)
= -3 * 6
= -18


7. -4(-11) 

= -4(-11) 
= 4 * 11
= 44

8. 32 / -8

= 32 / -8
= -4 


9. -25 / -5 

= -25 / -5 
= 25 / 5
= 5


10. -3 + |-4| 

= -3 + |-4| 
= -3 + 4
= 4 - 3
= 1


11. |-6| - 7 

= |-6| - 7 
= 6 - 7
= -1 

12. 90 / -30 

= 90 / -30 
= -3


13. -11 + 20 

= -11 + 20 
= 20 - 11
= 9

14. -6 - (-3)

= -6 - (-3)
= -6 + 3
= -3 


15. -3 + 2 + (-5)

= -3 + 2 + (-5)
= -3 + 2 - 5
= -1 - 5
= -6


16. -5 - 5 

= -5 - 5 
= -10


17. (-2)(-3)(-4) 

= (-2)(-3)(-4) 
= -2 * -3 * -4
= 6 * -4
= -24


18. (-4)(-8) 

= (-4)(-8) 
= -4 * -8
= 32

19. -3 + 1 - (-2) 

= -3 + 1 - (-2) 
= -2 - -2
= -2 + 2
= 0


20. (-1)(-1)(-1)(-1) 

= (-1)(-1)(-1)(-1) 
= -1 * -1 * -1 * -1
= 1 * -1 * -1
= 1 * 1
= 1

21. 1 + 6 * 3 / 2 - 2 

= 1 + 6 * 3 / 2 - 2 
= 1 + 18 / 2 -2
= 1 + 9 - 2
= 8

22. 12 / 3 * 2 - 1 

= 12 / 3 * 2 - 1 
= 4 * 2 - 1
= 8 - 1
= 7


23. 0 * 7 + 15 / 5 - 2 * 1

= 0 * 7 + 15 / 5 - 2 * 1
= 0 + 15 / 5 - 2 * 1
= 3 - 2 * 1
= 3 - 2
= 1

24. (-10) * 12 - 6 * 3

= (-10) * 12 - 6 * 3
= -120 - 6 * 3
= -120 - 18
= -138


25. |-5| + |-3| - |-2|

= |-5| + |-3| - |-2|
= 5 + 3 - 2
= 6

26. -|-3| + |7|

= -|-3| + |7|
= -3 + 7
= 7 - 3
= 4

