1. -7(x+2y-3)

= -7(x+2y-3)
= -7x-14y+21

2. 3x+4x+(x+2)

= 3x + 4x + (x+2)
= 7x+x+2
= 8x+2

3. 2(x+y)+7x+3

= 2(x+y)+7x+3
= 2x+2y+7x+3
= 9x + 2y + 3

4. -(-2x+1)+1

= -(-2x+1)+1
= 2x-1+1
= 2x

5. 7x-2y+5+(2x+5y-4)

= 7x - 2y + 5 + (2x +5y -4)
= 7x - 2y + 5 + 2x +5y -4
= 9x -2y +5y +2x +5 -4
= 9x +3y +1

6. (3x+5xy+2y)+(4-3xy-2x)

= (3x + 5xy + 2y) + (4 - 3xy -2x)
= 3x + 5xy +2y +4 -3xy -2x
= 3x - 2x +5xy - 3xy +2y +4
= x +2xy +2y + 4

7. (5y-2a+1)+2(y-3a-7)

= (5y - 2a +1) + 2(y - 3a - 7)
= 5y -2a +1 + 2y -6a -14 + 1
= 5y + 2y -2a - 6a - 14 + 1
= 7y -8a - 13

8. 3(2a-b)-4(b-2a)

= 3(2a - b) - 4(b - 2a))
= 6a - 3b -4b +8a
= 6a +8a -3b - 4b 
= 14a -7b

9. 2(7x-5+y)-(y+7)

= 2(7x - 5 + y) - (y + 7)
= 14x - 10 + 2y -y - 7
= 14x +y - 17

10. 5-2(x+2[3+x])

= 5 - 2(x + 2[3 + x])
= 5 - 2(x + 6 + 2x)
= 5 - 2x - 12 - 4x
= -4x - 2x + 5 - 12
= -6x - 7

11. x-{2x-2(1-x)}

= x - {2x - 2(1 - x)}
= x - {2x -2 + 2x}
= x - 2x + 2 -2x 
= x -4x + 2
= 3x + 2

12. 4-9(2x-3)+7(x-1)

= 4 - 9(2x - 3) + 7(x - 1)
= 4 - 18x + 27 + 7x - 7
= (-11x + 24) or (24 - 11x)

13. 3(x+4)+5x-8

= 3(x + 4) + 5x - 8
= 3x + 12 + 5x -8
= 8x + 12 - 8
= 8x + 4

14. 4x-[5-3(2x-6)]

= 4x - [5 - 3(2x - 6)]
= 4x - [5 - 6x + 18]
= 4x -5 +6x - 18
= 10x - 23