1. 2x-7 = 9-6x

:: 2x - 7 = 9 - 6x
:: 2x = 9 + 7 - 6x
:: 2x + 6x = 16
:: 8x = 16
:: x = 2

2. 2(x+1) - 3(4x-2) = 6x

:: 2(x + 1) - 3(4x - 2) = 6x
:: 2x + 2 - 12x + 6 = 6x
:: -10x + 8 = 6x
::  -16x = -8
:: x = 1/2

3. (x-3)/4 = 5

:: x - 3 = 20
:: x = 23

4. 20 - (3x/5) = x - 12

:: x = 32 - (3x / 5)
:: 5x = (32 * 5) - (3x / 5 * 5)
:: 5x = 160 - 3x
:: 8x = 160
:: x = 20

5. 2x - 9 = 5x - 15

:: 2x = 5x - 15 + 9
:: 2x - 5x = -6
:: -3x = -6
:: 3x = 6
:: x = 2

6. 2(x + 2) = 5 + ((x+1)/3))

:: 2x + 4 - 5 = (x+1)/3
:: 2x - 1 = (x+1)/3
:: 6x - 3 = x + 1
:: 5x = 4
:: x = 4/5

7. 15 - 3(9 - x) = x

:: 15 - 27 + 3x = x
:: -12 = -2x
:: x = 6

8. 3 - (5(x-1)/2) = x 

:: 3 - ((5x - 5) / 2) = x
:: 6 - 5x + 5 = 2x
:: 11 - 5x = 2x
:: 11 = 7x
:: x = 11 / 7

9. x - ((x-1)/4) = 0

:: x = ((x-1)/4)
:: 4x = x - 1
:: 3x = -1
:: x = -1/3

10. 1 - (x/2) = 5

:: 2 - x = 10
:: -x = 8
:: x = -8

11. -5w - 1 = -9w - 1

:: -1 = -9w + 5w - 1
:: -1 = -4w - 1
:: 1 = 4w + 1
:: 4w = 0
:: w = 0

12. 3(-2x + 1) = -6x - 7

:: -6x + 3 = -6x - 7
:: 0x = -10
:: 0 = -10, which is impossible; therefore, unsolveable
:: note that the solution in the book is different, but still returns unsolveable; I believe there is an error in their arithmetic, but the answer remains the same

13. 2(4a+1) = 4(2a-1) + 6

:: 8a + 2 = 8a - 4 + 6
:: 0a = 6 - 4 - 2
:: 0a = 0
:: 0 = 0
:: therefore, true for all real numbers (identity)

14. 3(z + 5) - 2z = ((z-1)/2) + 17

:: 3z + 15 - 2z = ((z-1)/2) + 17
:: z = (z-1)/2  + 17 - 15
:: 2z = z - 1 + 4
:: z = 3

15. 13 - (2y + 2) = 2(y + 2) + 3y

:: 11 - 2y = 2y +4 + 3y
:: 11 - 4 = 2y + 3y + 2y
:: 7 = 7y
:: y = 1

16. 3x + 4(x - 2) = x - 5 + 3(2x-1)

:: 3x +4x - 8 = x - 5 + 6x - 3
:: 7x - 8 = 7x - 8
:: 7x - 7x = -8 + 8
:: 0 = 0, therefore true for all real numbers (identity)

17. 2c + 3(c + 2) = 5c + 11

:: 2c + 3c + 6 = 5c + 11
:: 5c + 6 = 5c + 11
:: cannot be equal, therefore no solution

18. 2[2 - x - (2x-5)] = 11 - x

:: 2[2 - x - 2x + 5] = 11 - x
:: 4 - 2x -4x + 10 = 11 - x
:: 14 - 6x = 11 - x
:: 14 - 5x = 11
:: 14 - 11 = 5x
:: 3 = 5x
:: x = 3/5