1. 1 = 5/x

:: 1 * x = 5/x *x
:: x = 5

2. (x-3)/2 = (2x+4)/5

:: (x-3) * 5 = (2x+4) *2
:: 5x - 15 = 4x + 8
:: x = 8 + 15
:: x = 23

3. 6/(x-2) = -3

:: 6/(x-2) * (x-2) = -3(x-2)
:: 6 = -3x + 6
:: -3x = 0
:: x = 0

4. (3x - 3) / (x - 1) = 2

:: 3x -3 / (x - 1) * (x - 1) = 2(x - 1)
:: 3x - 3 = 2x - 2
:: 3x - 3 = 2x - 2
:: x = 1

:: check answer, because denominator has a variable
::
:: 3 - 3 /  1-1 = 2
:: cannot divide by zero, so the solution i undefined (no solution)

5. x/2 = (x+6) / 3

:: x * 3 = (x+6) * 2
:: 3x = 2x + 12
:: x = 12

6. 3 / x = 4 / (x - 2)

:: 3(x-2) = 4x
:: 3x - 6 = 4x
:: -6 = x
:: x = -6

7. 4/(x+3) = 1/(x-3)

:: 4(x-3) = 1(x+3)
:: 4x - 12 = x + 3
:: 3x = 15
:: x = 5

8. (5 - 2x) / (x-1) = -2

:: 5 - 2x = -2x + 2
:: -2x = -2x -3
:: 0 = -3 ==  undefined (no solution)

9. (x + 3) / (x - 2) = 2

:: x + 3 = 2x - 4
:: 3 = x - 4
:: x = 7

10. (4 / 5)x - (1 / 4) = (-3 / 2)x20

:: 20 * ((4/5)x - (1/4)) = 20((-3/2)x)   <-- find common denominator, multiply numerator by it
:: (20 * 4 * x)/5 - 20/4 = (20 * -3)/2 * x
:: 4 * 4 * x - 5 = -30x
::16x -5 = -30x
:: -46x = -5
:: x = 5/46

11. 5 + (3 + x)/x = (5/x)

:: 5x + 3 + x = 5
:: 6x = 2
:: x = 1/3

12. 4/(x-2) - (1/x) = 5 / (x-2)

:: (4/(x-2)) - (1/x) = 5 / (x - 2) <-- common denominator is x(x-2), so multiply numerators by it
:: (4 * x(x-2)/(x-2)) - (1x-2/x) = (5 * x(x-2)) / (x-2)
:: 4x - x - 2 = 5x
:: 3x +2 = 5x
:: 2x = 22
:: x = 1  <-- now have to check, since denominator had a variable

:: 4/(1-2) - 1/1 = 5/1-2 
:: 4/-1 - 1/1 = 5/1-1
:: -4 - 1 = -5
:: -5 = -5 <-- true, therefore x = -1